src/Tactics.v
@@ -159,3 +159,10 @@ Theorem refine_If_Then_Else_bool :
     (if b then refine cpst res else refine cpse res)
       <-> refine (If b Then cpst Else cpse) res.
 Proof. split; intros; destruct b; auto. Qed.
+
+Lemma refine_ret_eq_r : forall A (a b : A), refine (ret a) (ret b) -> a = b.
+Proof.
+  intros.
+  specialize (H b (ReturnComputes b)).
+  apply Return_inv; assumption.
+Qed.
